middleware/authUtils.js
@@ -1,0 +1,5 @@
+function isAuthorized(username, password, adminUsername, adminPassword) {
+  return username === adminUsername && password === adminPassword;
+}
+
+module.exports = { isAuthorized };
